Make `tick` fallible
The inciting reason to do this was to be able to model window bus
errors; it could also be useful for disallowing certain actions, though
(e.g. making sure the I2C peripheral is never set to target mode).

Whether or not the latter use case is supported comes down to whether
the `rsp.error <=> ISL (cheshire_run ...)` clause is preserved, or if
it's changed to `rsp.error ==> ISL (cheshire_run ...)`.

util/gen_regs_comm.py
@@ -253,10 +253,12 @@ End
 (* This probably shouldn't go here but I don't want to create a whole new file
  * just for this. *)
 Theorem {ip.name}_tick_hwro_unchanged:
-  {" /\\\n  ".join(f"({ip.name}_tick notif st).regs.{name(reg)}.{name(field)} = st.regs.{name(reg)}.{name(field)}" for reg in regs for field in reg.fields if not reg.hwext and not field.hwaccess.allows_write())}
+  {ip.name}_tick notif st = INR st' ==>
+  {" /\\\n  ".join(f"st'.regs.{name(reg)}.{name(field)} = st.regs.{name(reg)}.{name(field)}" for reg in regs for field in reg.fields if not reg.hwext and not field.hwaccess.allows_write())}
 Proof
   simp [{ip.name}_tick_def]
-  >> rpt strip_tac
+  >> disch_then (assume_tac o GSYM)
+  >> simp []
   >> rpt IF_CASES_TAC
   >> simp []
 QED
